

Let there be observations x_1, x_2, \dots, x_n and weights w_1, \dots, w_n . Without loss of generality, $\sum_i w_i = 1$.

$$\begin{aligned} \sum_{i \neq j} \frac{1}{2} w_i w_j (x_i - x_j)^2 &= \sum_{i \neq j} \frac{1}{2} (w_i x_i^2 w_j + w_j x_j^2 w_i - 2w_i x_i w_j x_j) \\ &= \sum_i \frac{1}{2} w_i (1 - w_i) x_i^2 + \sum_j \frac{1}{2} w_j (1 - w_j) x_j^2 - \sum_{i \neq j} w_i x_i w_j x_j \\ &= \sum_i w_i (1 - w_i) x_i^2 - \sum_{i \neq j} w_i x_i w_j x_j. \end{aligned}$$

As $(\sum_i w_i x_i)^2 = \sum_i w_i^2 x_i^2 + \sum_{i \neq j} w_i x_i w_j x_j$, this gives

$$\begin{aligned} \sum_{i \neq j} \frac{1}{2} w_i w_j (x_i - x_j)^2 &= \sum_i w_i x_i^2 - (\sum_i w_i x_i)^2 \\ &= \sum_i w_i x_i^2 - 2(\sum_i w_i x_i)^2 + (\sum_i w_i x_i)^2 \\ &= \sum_i w_i x_i^2 - 2 \sum_i w_i x_i (\sum_j w_j x_j) + \sum_i w_i (\sum_j w_j x_j)^2 \\ &= \sum_i w_i [x_i - (\sum_j w_j x_j)]^2 \\ &= \text{Var}_w(x). \end{aligned}$$

Similarly, I think,

$$\sum_{i \neq j} \frac{1}{2} w_i w_j (x_i - x_j)(y_i - y_j) = \sum_i w_i x_i y_i - (\sum_i w_i x_i)(\sum_i w_i y_i) = \text{Cov}_w(x, y).$$